AbstractPlatform/Types.bpl
@@ -170,8 +170,8 @@ function tap_proof_op_valid_in_enclave(o : tap_proof_op_t) : bool
 {
     // false
     // o == tap_proof_op_pause        
-    // o == tap_proof_op_compute      
-    o == tap_proof_op_exit      
+    o == tap_proof_op_compute      
+    // o == tap_proof_op_exit      
 }
 
 function tap_proof_op_valid_in_privileged (o : tap_proof_op_t) : bool
